\chapter{Useful Identities}\label{app:useful identities}
        \section{\texorpdfstring{\(\abs{z + w}^2 = \abs{z}^2 + \abs{w}^2 + 2\Re(zw^*)\)}{|z+w|2 = |z|2 + |w|2 + 2Re(zw*)}}
        Let \(z, w \in \complex\). Then
        \begin{align}
            \abs{z + w}^2 &= (z + w)(z + w)^*\\
            &= (z + w)(z^* + w^*)\\
            &= zz^* + ww^* + zw^* + z^*w\\
            &= \abs{z}^2 + \abs{w}^2 + zw^* + z^*w.
        \end{align}
        Identifying \(z^*w = (zw^*)^*\) it is clear that if \(zw^* = x + iy\) then \(zw^* + z^*w = x + iy + x - iy = 2x = 2\Re(zw^*)\), and hence
        \begin{equation}
            \abs{z + w}^2 = \abs{z}^2 + \abs{w}^2 + 2\Re(zw^*).
        \end{equation}