\section{Sum of \texorpdfstring{\(k\)}{k} From 0 to \texorpdfstring{\(n\)}{n} Proof}\label{sec:proof sum 0 to n of r is 0.5 n(n+1)}
    \begin{theorem}{}{}
        For \(n \in \naturals\)
        \[\sum_{r=0}^{n} r = \frac{1}{2}n(n + 1).\]
    \end{theorem}
    \begin{proof}
        We will prove this by induction.
        First note that
        \[\sum_{r=0}^{0}r\]
        is the empty sum which is defined to be zero by convention.
        Now suppose that this result holds for some \(k \in \naturals\), that is
        \[\sum_{r = 0}^{k} r = \frac{1}{2}k(k + 1).\]
        Then
        \begin{align*}
            \sum_{r = 0}^{k + 1} r &= \sum_{r = 0}^{k} r + (k + 1)\\
            &= \frac{1}{2}k(k + 1) + (k + 1)\\
            &= (k + 1)\left[\frac{1}{2}k + 1\right]\\
            &= \frac{1}{2}(k + 1)(k + 2)
        \end{align*}
        which is exactly what we would expect if the hypothesis held for \(k + 1\).
        Hence by induction
        \[\sum_{r=0}^{n} r = \frac{1}{2}n(n + 1)\]
        holds for all \(n\in\naturals\).
    \end{proof}